methods done to pass level

G20735820CarPark.dfy
@@ -1,50 +1,74 @@
 class {:autocontracts} CarPark{
-    const capacity : int; //total capacity car park can take
+    const capacity : int := 10; //total capacity car park can take
+    const rCapacity : int := 10;
     var urArea : set<int>; //the car park, will fill up with ids of car
     var rArea : set<int>;
-    var arbitraryVal : int;
+    var subs: set<int>;
+    const fullSpaceMargin: int := 5; //car park considered full when 5 spaces left
+    var isWeekend: bool;
     constructor()
     ensures urArea == {}
     ensures rArea == {}
     ensures capacity > 0;
+    ensures rCapacity > 0;
+    ensures isWeekend == false
     {
-        capacity := 20;
+        //capacity := 20;
         rArea := {};
         urArea := {};
+        isWeekend := false;
     }
 
     predicate Valid()
     reads this
     {
-        (|urArea| <= capacity) //- minSpaces)
+        (|urArea| <= capacity) && (|rArea| <= capacity) //- minSpaces)
     }
 
     method EnterCarPark(carId : int)
-    requires |urArea| < capacity; //- minSpaces;
-    //requires Valid();
-    modifies this
-    //ensures Valid();
+    requires |urArea| < capacity - fullSpaceMargin; //- minSpaces;
+    modifies `urArea
     ensures urArea == old(urArea) + {carId}
     {
         //if the amount of cars is less than capacity then insert the car
         urArea := urArea + {carId};
     }
 
-    /*method LeaveCarPark(carId : int)
-    modifies this
-    {
-        urArea := urArea - {carId};
-    }*/
-
-    method LeaveCarPark()
+    method LeaveCarPark(carId : int)
     requires |urArea| > 0
-    modifies this
+    requires carId in urArea || carId in rArea
+    modifies `urArea, `rArea
+    ensures urArea == old(urArea) - {carId}
+    {
+        if(carId in urArea){
+            urArea := urArea - {carId};
+        }else if(carId in rArea){
+            rArea := rArea - {carId};
+        }
+    }
+
+    method CheckAvailability()
+    ensures urArea == old(urArea)
+    ensures rArea == old(rArea)
+    ensures isWeekend == old(isWeekend)
+    ensures subs == old(subs)
+    {
+        if(isWeekend){
+            print capacity - |rArea|;
+        }else{
+            print capacity - |urArea|;
+        }
+    }
+
+    /*method LeaveCarPark()
+    requires |urArea| > 0
+    modifies `urArea
     ensures |urArea| == |old(urArea)| - 1
     {
         var leavingCarId : int; //need to make a local var as dafny assume clause only supports local var currently
         leavingCarId :| leavingCarId in urArea; // taken from lecture 17 finds arbitrary value in the set to remove
         urArea := urArea - {leavingCarId}; //remove the arbitrary value from the set
-    }
+    }*/
 }
 
 method Main(){
@@ -56,21 +80,23 @@ method Main(){
     cp.EnterCarPark(3);
     print cp.urArea;
 
-    cp.LeaveCarPark();
-    cp.LeaveCarPark();
-    cp.LeaveCarPark();
+    print "Checking avail: ";
+    cp.CheckAvailability();
+    print "\n";
+
+    cp.LeaveCarPark(1);
+    cp.LeaveCarPark(2);
+    cp.LeaveCarPark(3);
     
     print cp.urArea;
 
+    cp.EnterCarPark(2);
+    cp.EnterCarPark(3);
 
-    cp.EnterCarPark(4);
-    cp.EnterCarPark(5);
-    cp.EnterCarPark(6);
     print cp.urArea;
 
-    cp.LeaveCarPark();
-    cp.LeaveCarPark();
-    cp.LeaveCarPark();
-    //cp.LeaveCarPark(2);
-    print cp.urArea;
+    print "Checking avail: ";
+    cp.CheckAvailability();
+    print "\n";
+
 }
